theory/Util.v
@@ -1,4 +1,6 @@
 Set Warnings "-notation,-overridden,-parsing".
+Require Import Coq.Init.Nat.
+Require Import Ascii.
 Require Import Coq.Strings.String.
 Open Scope string_scope.
 Open Scope list_scope.
@@ -16,19 +18,63 @@ Fixpoint map {X Y : Type} (f: X->Y) (l: list X) : (list Y) :=
   | h :: t => (f h) :: (map f t)
   end.
 
-Definition beq_string (s1 : string) (s2 : string) :=
-  if string_dec s1 s2 then true else false.
+Definition beq_nat := PeanoNat.Nat.eqb.
+
+Fixpoint beq_string (s1 : string) (s2 : string) :=
+  match s1 with
+  | "" => match s2 with
+         | "" => true
+         | _ => false
+         end
+  | String a s1' => match s2 with
+                   | "" => false
+                   | String b s2' =>
+                     let a' := nat_of_ascii a in
+                     let b' := nat_of_ascii b in
+                     andb (beq_nat a' b') (beq_string s1' s2')
+                   end
+  end.
+
+(* Definition beq_string (s1 : string) (s2 : string) := *)
+(*   if string_dec s1 s2 then true else false. *)
 
 Lemma beq_string_refl : forall (s : string),
     beq_string s s = true.
 Proof.
-  intros. induction s as [| a s].
-  - reflexivity.
-  - unfold beq_string. destruct (string_dec (String a s) (String a s)).
-    + reflexivity.
-    + destruct n. reflexivity.
+  intros. induction s as [| a s]; try reflexivity.
+  - simpl. rewrite <- EqNat.beq_nat_refl. assumption.
 Qed.
 
+Lemma beq_string_empty_r : forall (s : string),
+    beq_string s "" = true -> s = "".
+Proof.
+  intros. induction s; (try reflexivity; inversion H).
+Qed.
+
+Lemma beq_string_empty_l : forall (s : string),
+    beq_string "" s = true -> s = "".
+Proof.
+  intros. induction s; (try reflexivity; inversion H).
+Qed.
+
+Lemma beq_string_correct : forall (s : string) (t : string),
+    beq_string s t = true -> s = t.
+Proof.
+  intro s. induction s.
+  - intros. rewrite (beq_string_empty_l _ H). reflexivity.
+  - destruct t.
+    + discriminate.
+    + admit.
+Admitted.
+  
+Lemma beq_string_comm : forall (s : string) (t : string),
+    beq_string s t = true -> beq_string t s = true.
+Proof.
+  intros. generalize dependent s. induction t.
+  - intros. rewrite (beq_string_empty_r _ H). reflexivity.
+  - admit.
+Admitted.
+      
 Fixpoint beq_string_list (ss : list string) (ss': list string) :=
   match ss with
   | [] => match ss' with
@@ -48,4 +94,3 @@ Proof.
   - reflexivity.
   - simpl. rewrite beq_string_refl. assumption.
 Qed.
-
